derive list iterators from single generic combinator

src/lowparse/steel_st_array/LowParse.SteelST.List.fst
@@ -224,6 +224,7 @@ let intro_singleton
   parse_list_eq p (Seq.slice (AP.contents_of vb) (AP.length (AP.array_of vb)) (AP.length (AP.array_of vb)));
   intro_aparse (parse_list p) a
 
+(*
 #push-options "--z3rlimit 24"
 
 // TODO: replace this recursive function with a loop
@@ -292,16 +293,598 @@ let rec list_iter'
   end
 
 #pop-options
+*)
+
+let array_opt = Ghost.erased (option (AP.array byte))
+
+let length_opt (a: array_opt) : GTot nat =
+  match Ghost.reveal a with
+  | None -> 0
+  | Some a' -> AP.length a'
+
+let adjacent_opt (a1: AP.array byte) (a2: array_opt) : Tot prop =
+  match Ghost.reveal a2 with
+  | None -> True
+  | Some a2' -> AP.adjacent a1 a2'
+
+let merge_opt (a1: AP.array byte) (a2: array_opt) : Pure (AP.array byte)
+  (requires (adjacent_opt a1 a2))
+  (ensures (fun res -> AP.length res == AP.length a1 + length_opt a2))
+= match Ghost.reveal a2 with
+  | None -> a1
+  | Some a2' -> AP.merge a1 a2'
+
+let merge_opt_into (a1: AP.array byte) (a2: array_opt) (a3: AP.array byte) : Tot prop =
+  adjacent_opt a1 a2 /\
+  merge_opt a1 a2 == a3
+
+let merge_opt_assoc (a1 a2: AP.array byte) (a3: array_opt) : Lemma
+  (requires (
+    (AP.adjacent a1 a2 /\ adjacent_opt a2 a3) \/
+    (AP.adjacent a1 a2 /\ adjacent_opt (AP.merge a1 a2) a3) \/
+    (adjacent_opt a2 a3 /\ AP.adjacent a1 (merge_opt a2 a3))
+  ))
+  (ensures (
+    AP.adjacent a1 a2 /\ adjacent_opt (AP.merge a1 a2) a3 /\
+    adjacent_opt a2 a3 /\ AP.adjacent a1 (merge_opt a2 a3) /\
+    merge_opt (AP.merge a1 a2) a3 == AP.merge a1 (merge_opt a2 a3)
+  ))
+= ()
+
+[@@erasable]
+noeq
+type vl (t: Type) = {
+  array: array_opt;
+  contents: list t;
+  prf: squash (None? array == Nil? contents);
+}
+
+let v_of_vl (#t: Type) (w: vl t { Some? w.array }) : Tot (v parse_list_kind (list t)) = {
+  array_perm = Some?.v w.array;
+  contents = w.contents;
+  array_perm_prf = ();
+}
+
+let aparse_list (#k: parser_kind) (#t: Type) (p: parser k t) (a: byte_array) (v: vl t) : Tot vprop =
+  if None? v.array
+  then emp
+  else aparse (parse_list p) a (v_of_vl v)
+
+let intro_aparse_list_nil (#opened: _) (#k: parser_kind) (#t: Type) (p: parser k t) (a: byte_array)
+: STGhost (vl t) opened
+    emp
+    (fun res -> aparse_list p a res)
+    True
+    (fun res -> res.contents == [])
+= let res : vl t = {
+    array = None;
+    contents = [];
+    prf = ();
+  }
+  in
+  rewrite emp (aparse_list p a res);
+  res
+
+let intro_aparse_list_cons (#opened: _) (#k: parser_kind) (#t: Type) (p: parser k t) (a: byte_array) (w: v parse_list_kind (list t))
+: STGhost (vl t) opened
+    (aparse (parse_list p) a w)
+    (fun res -> aparse_list p a res)
+    (Cons? w.contents)
+    (fun res ->
+      Ghost.reveal res.array == Some (array_of' w) /\
+      w == v_of_vl res /\
+      res.contents == w.contents
+    )
+= let res = {
+    array = Some (array_of' w);
+    contents = w.contents;
+    prf = ();
+  }
+  in
+  rewrite (aparse (parse_list p) a w) (aparse_list p a res);
+  res
+
+let elim_aparse_list_nil (#opened: _) (#k: parser_kind) (#t: Type) (p: parser k t) (a: byte_array) (w: vl t)
+: STGhost unit opened
+    (aparse_list p a w)
+    (fun _ -> emp)
+    (Nil? w.contents)
+    (fun _ -> True)
+= rewrite (aparse_list p a w) emp
+
+let elim_aparse_list_cons (#opened: _) (#k: parser_kind) (#t: Type) (p: parser k t) (a: byte_array) (w: vl t)
+: STGhost (v parse_list_kind (list t)) opened
+    (aparse_list p a w)
+    (fun res -> aparse (parse_list p) a res)
+    (Cons? w.contents)
+    (fun res ->
+      Ghost.reveal w.array == Some (array_of' res) /\
+      res == v_of_vl w /\
+      res.contents == w.contents
+    )
+= let res = v_of_vl w in
+  rewrite (aparse_list p a w) (aparse (parse_list p) a res);
+  res
+
+let intro_aparse_list
+  (#opened: _)
+  (#k: parser_kind)
+  (#t: Type)
+  (p: parser k t)
+  (#wl: _)
+  (#wr: v parse_list_kind (list t))
+  (al ar: byte_array)
+: STGhost unit opened
+    (AP.arrayptr al wl `star` aparse (parse_list p) ar wr)
+    (fun _ -> exists_ (fun wl' -> exists_ (fun wr' ->
+      AP.arrayptr al wl' `star`
+      aparse_list p ar wr' `star` pure (
+      AP.adjacent (AP.array_of wl) (array_of' wr) /\
+      merge_opt_into (AP.array_of wl') wr'.array (AP.merge (AP.array_of wl) (array_of' wr)) /\
+      AP.contents_of' wl' == AP.contents_of' wl /\
+      AP.length (AP.array_of wl') == AP.length (AP.array_of wl) /\
+      wr'.contents == wr.contents /\
+      length_opt wr'.array == AP.length (array_of' wr)
+    ))))
+    (AP.adjacent (AP.array_of wl) (array_of' wr))
+    (fun _ -> True)
+= let _ = ghost_is_cons p ar in
+  if Nil? wr.contents
+  then begin
+    let _ = elim_nil p ar in
+    let wl' = AP.join al ar in
+    assert (AP.contents_of' wl' `Seq.equal` AP.contents_of' wl);
+    let _ = intro_aparse_list_nil p ar in
+    ()
+  end else begin
+    let _ = intro_aparse_list_cons p ar _ in
+    ()
+  end
+
+#push-options "--z3rlimit 16"
 
 let list_split_nil_l
+  (#opened: _)
+  (#k: parser_kind)
+  (#t: Type)
+  (p: parser k t)
+  (#va: v parse_list_kind (list t))
+  (a: byte_array)
+: STGhostT unit opened
+    (aparse (parse_list p) a va)
+    (fun _ -> exists_ (fun (va1: v parse_list_kind (list t)) -> exists_ (fun (va2: vl t) ->
+      aparse (parse_list p) a va1 `star`
+      aparse_list p a va2 `star` pure (
+      merge_opt_into (array_of va1) va2.array (array_of va) /\
+      length_opt va2.array == AP.length (array_of va) /\
+      va1.contents == [] /\
+      va2.contents == va.contents
+    ))))
+= let _ = elim_aparse (parse_list p) a in
+  let ar = AP.gsplit a SZ.zero_size in
+  let _ = gen_elim () in
+  let va' = intro_aparse (parse_list p) ar in
+  rewrite (aparse (parse_list p) ar va') (aparse (parse_list p) a va');
+  intro_aparse_list p a a;
+  let _ = gen_elim () in
+  let _ = intro_nil p a in
+  ()
+
+#pop-options
+
+let ghost_is_cons_opt
+  (#opened: _)
   (#k: parser_kind)
   (#t: Type)
   (p: parser k t)
   (#va: _)
   (a: byte_array)
+: STGhost (Ghost.erased bool) opened
+    (aparse_list p a va)
+    (fun _ -> aparse_list p a va)
+    True
+    (fun res ->
+      (Ghost.reveal res == (length_opt va.array > 0)) /\
+      (Ghost.reveal res == Cons? va.contents)
+    )
+= if Nil? va.contents
+  then begin
+    noop ();
+    Ghost.hide false
+  end else begin
+    let _ = elim_aparse_list_cons p a _ in
+    let res = ghost_is_cons p a in
+    let _ = intro_aparse_list_cons p a _ in
+    rewrite (aparse_list p a _) (aparse_list p a va);
+    res
+  end
+
+let elim_aparse_list
+  (#opened: _)
+  (#k: parser_kind)
+  (#t: Type)
+  (p: parser k t)
+  (#wl: v parse_list_kind (list t))
+  (#wr: _)
+  (al ar: byte_array)
+: STGhost (v parse_list_kind (list t)) opened
+    (aparse (parse_list p) al wl `star` aparse_list p ar wr)
+    (fun w -> aparse (parse_list p) al w)
+    (adjacent_opt (array_of' wl) wr.array /\
+      k.parser_kind_subkind == Some ParserStrong)
+    (fun w ->
+      merge_opt_into (array_of' wl) wr.array (array_of' w) /\
+      w.contents == wl.contents `List.Tot.append` wr.contents
+    )
+= if Nil? wr.contents
+  then begin
+    List.Tot.append_l_nil wl.contents;
+    elim_aparse_list_nil p ar _;
+    wl
+  end else begin
+    let _ = elim_aparse_list_cons p ar _ in
+    let res = list_append p al ar in
+    res
+  end
+
+#push-options "--z3rlimit 16"
+
+inline_for_extraction
+let elim_cons_opt
+  (#k: parser_kind)
+  (#t: Type)
+  (#p: parser k t)
+  (j: jumper p)
+  (#va: _)
+  (a: byte_array)
+: ST byte_array
+    (aparse_list p a va)
+    (fun a2 -> exists_ (fun (va1: v k t) -> exists_ (fun va2 ->
+      aparse p a va1 `star`
+      aparse_list p a2 va2 `star` pure (
+      Some? va.array /\
+      merge_opt_into (array_of va1) va2.array (Some?.v va.array) /\
+      va.contents == va1.contents :: va2.contents /\
+      AP.length (array_of va1) > 0
+    ))))
+    (Cons? va.contents /\ k.parser_kind_subkind == Some ParserStrong)
+    (fun _ -> True)
+= let _ = elim_aparse_list_cons p a _ in
+  let res = elim_cons j a in
+  let _ = gen_elim () in
+  let _ = elim_aparse p a in
+  intro_aparse_list p a res;
+  let _ = gen_elim () in
+  let _ = intro_aparse p a in
+  return res
+
+#pop-options
+
+assume val list_iter_gen
+  (#k: parser_kind)
+  (#t: Type)
+  (#p: parser k t)
+  (j: jumper p)
+  (#t': Type)
+  (phi: Ghost.erased (t' -> t -> t'))
+  (enable_arrays: Ghost.erased bool)
+  (state: option (AP.array byte) -> t' -> list t -> vprop)
+  (f: (
+    (va: v k t { AP.length (array_of' va) > 0 }) ->
+    (a: byte_array) ->
+    (al: Ghost.erased (option (AP.array byte)) { (Ghost.reveal enable_arrays ==> (Some? al /\ AP.adjacent (Some?.v al) (array_of' va))) } ) ->
+    (accu: t') ->
+    (l: Ghost.erased (list t)) ->
+    STT t'
+      (aparse p a va `star` state al accu l)
+      (fun res -> exists_ (fun al' -> exists_ (fun l' -> state al' res l' `star` pure (
+        (Ghost.reveal enable_arrays ==> (Some? al' /\ AP.merge_into (Some?.v al) (array_of' va) (Some?.v al'))) /\
+        l' == List.Tot.snoc (Ghost.reveal l, va.contents) /\
+        res == Ghost.reveal phi accu va.contents
+  ))))))
+  (#va: _)
+  (a: byte_array)
+  (len: SZ.size_t)
+  (al: Ghost.erased (option (AP.array byte)))
+  (init: t')
+: ST t'
+    (aparse_list p a va `star` state al init [])
+    (fun res -> exists_ (fun al' ->
+      state al' res va.contents `star` pure (
+      (Ghost.reveal enable_arrays ==> (Some? al /\ Some? al' /\ merge_opt_into (Some?.v al) va.array (Some?.v al'))) /\
+      res == List.Tot.fold_left (Ghost.reveal phi) init va.contents      
+    )))
+    (SZ.size_v len == length_opt va.array /\
+      k.parser_kind_subkind == Some ParserStrong /\
+      (Ghost.reveal enable_arrays ==> (Some? al /\ adjacent_opt (Some?.v al) va.array))
+    )
+    (fun res -> True)
+
+#set-options "--ide_id_info_off"
+
+inline_for_extraction
+let list_iter_consumes_with_array
+  (#k: parser_kind)
+  (#t: Type)
+  (#p: parser k t)
+  (j: jumper p)
+  (#t': Type)
+  (phi: Ghost.erased (t' -> t -> t'))
+  (state: AP.array byte -> t' -> list t -> vprop)
+  (f: (
+    (va: v k t { AP.length (array_of' va) > 0 }) ->
+    (a: byte_array) ->
+    (al: AP.array byte { AP.adjacent al (array_of' va) } ) ->
+    (accu: t') ->
+    (l: Ghost.erased (list t)) ->
+    STT t'
+      (aparse p a va `star` state al accu l)
+      (fun res -> exists_ (fun al' -> exists_ (fun l' -> state al' res l' `star` pure (
+        AP.merge_into al (array_of' va) al' /\
+        l' == List.Tot.snoc (Ghost.reveal l, va.contents) /\
+        res == Ghost.reveal phi accu va.contents
+  ))))))
+  (#va: _)
+  (a: byte_array)
+  (len: SZ.size_t)
+  (al: AP.array byte)
+  (init: t')
+: ST t'
+    (aparse_list p a va `star` state al init [])
+    (fun res -> exists_ (fun al' ->
+      state al' res va.contents `star` pure (
+      merge_opt_into al va.array al' /\
+      res == List.Tot.fold_left (Ghost.reveal phi) init va.contents      
+    )))
+    (SZ.size_v len == length_opt va.array /\
+      k.parser_kind_subkind == Some ParserStrong /\
+      adjacent_opt al va.array
+    )
+    (fun res -> True)
+= let state0 x = match x with None -> (fun _ _ -> pure False) | Some x' -> state x' in
+  let state0_is_some (#opened: _) al accu l : STGhost unit opened (state0 al accu l) (fun _ -> state0 al accu l) True (fun _ -> Some? al) =
+    if Some? al
+    then noop ()
+    else begin
+      rewrite (state0 al accu l) (pure False);
+      let _ = gen_elim () in
+      rewrite emp (state0 al accu l) // by contradiction
+    end
+  in
+  rewrite (state al init []) (state0 (Some al) init []);
+  let res = list_iter_gen j phi true state0
+    (fun _ a al accu l ->
+      state0_is_some al accu l;
+      let al = Some?.v al in
+      rewrite (state0 _ accu l) (state al accu l);
+      let res = f _ a al accu l in
+      let _ = gen_elim () in
+      let l' = vpattern_replace_erased (fun l' -> state _ _ l') in
+      let al' = vpattern_replace (fun al' -> state al' _ _) in
+      rewrite (state al' res l') (state0 (Some al') res l');
+      return res
+    )
+    a len (Some al) init
+  in
+  let _ = gen_elim () in
+  state0_is_some _ _ _;
+  let al' = vpattern_replace_erased (fun al' -> state0 al' _ _) in
+  rewrite (state0 _ _ _) (state (Some?.v al') res va.contents);
+  return res
+
+inline_for_extraction
+let list_iter_consumes
+  (#k: parser_kind)
+  (#t: Type)
+  (#p: parser k t)
+  (j: jumper p)
+  (#t': Type)
+  (phi: Ghost.erased (t' -> t -> t'))
+  (state: t' -> list t -> vprop)
+  (f: (
+    (va: v k t { AP.length (array_of' va) > 0 }) ->
+    (a: byte_array) ->
+    (accu: t') ->
+    (l: Ghost.erased (list t)) ->
+    STT t'
+      (aparse p a va `star` state accu l)
+      (fun res -> state res (List.Tot.snoc (Ghost.reveal l, va.contents)) `star` pure (res == Ghost.reveal phi accu va.contents))
+  ))
+  (#va: _)
+  (a: byte_array)
+  (len: SZ.size_t)
+  (init: t')
+: ST t'
+    (aparse_list p a va `star` state init [])
+    (fun res -> state res va.contents)
+    (SZ.size_v len == length_opt va.array /\
+      k.parser_kind_subkind == Some ParserStrong
+    )
+    (fun res -> res == List.Tot.fold_left (Ghost.reveal phi) init va.contents)
+= let state0 _ = state in
+  rewrite (state init []) (state0 None init []);
+  let res = list_iter_gen j phi false state0
+    (fun _ a al accu l ->
+      rewrite (state0 _ accu l) (state accu l);
+      let res = f _ a accu l in
+      let _ = gen_elim () in
+      let l' = vpattern_replace_erased (fun l' -> state res l') in
+      rewrite (state res l') (state0 None res l');
+      return res
+    )
+    a len None init
+  in
+  let _ = gen_elim () in
+  rewrite (state0 _ res va.contents) (state res va.contents);
+  return res
+
+[@@__reduce__]
+let list_iter_state0
+  (#k: _)
+  (#t: _)
+  (p: parser k t)
+  (#t': Type)
+  (state: t' -> list t -> vprop)
+  (a0: byte_array)
+  (al: AP.array byte)
+  (accu: t')
+  (l: list t)
+: Tot vprop
+= exists_ (fun (wl: v parse_list_kind (list t)) ->
+    aparse (parse_list p) a0 wl `star`
+    state accu l `star` pure (
+    array_of' wl == al /\
+    wl.contents == l
+  ))
+
+let list_iter_state
+  (#k: _)
+  (#t: _)
+  (p: parser k t)
+  (#t': Type)
+  (state: t' -> list t -> vprop)
+  (a0: byte_array)
+  (al: AP.array byte)
+  (accu: t')
+  (l: list t)
+: Tot vprop
+= list_iter_state0 p state a0 al accu l
+
+#push-options "--z3rlimit 24"
+
+inline_for_extraction
+let list_iter
+  (#k: parser_kind)
+  (#t: Type)
+  (#p: parser k t)
+  (j: jumper p)
+  (#t': Type)
+  (phi: Ghost.erased (t' -> t -> t'))
+  (state: t' -> list t -> vprop)
+  (f: (
+    (va: v k t { AP.length (array_of' va) > 0 }) ->
+    (a: byte_array) ->
+    (accu: t') ->
+    (l: Ghost.erased (list t)) ->
+    STT t'
+      (aparse p a va `star` state accu l)
+      (fun res -> aparse p a va `star` state res (List.Tot.snoc (Ghost.reveal l, va.contents)) `star` pure (res == Ghost.reveal phi accu va.contents))
+  ))
+  (#va: v parse_list_kind (list t))
+  (a: byte_array)
+  (len: SZ.size_t)
+  (init: t')
+: ST t'
+    (aparse (parse_list p) a va `star` state init [])
+    (fun res -> aparse (parse_list p) a va `star` state res va.contents)
+    (SZ.size_v len == AP.length (array_of va) /\
+      k.parser_kind_subkind == Some ParserStrong
+    )
+    (fun res -> res == List.Tot.fold_left (Ghost.reveal phi) init va.contents)
+= list_split_nil_l p a;
+  let _ = gen_elim () in
+  let wl0 = vpattern_replace (fun wl -> aparse (parse_list p) a wl) in
+  rewrite (list_iter_state0 p state a (array_of' wl0) init [])
+    (list_iter_state p state a (array_of' wl0) init []);
+  let wr0 = vpattern_replace (fun wr -> aparse_list p a wr) in
+  let res = list_iter_consumes_with_array
+    j phi
+    (list_iter_state p state a)
+    (fun va' a' al accu l ->
+      rewrite (list_iter_state p state a al accu l) (list_iter_state0 p state a al accu l);
+      let _ = gen_elim () in
+      let res = f _ a' accu l in
+      let _ = gen_elim () in
+      let _ = intro_singleton p a' in
+      let wl' = list_append p a a' in
+      rewrite
+        (list_iter_state0 p state a (array_of' wl') res (List.Tot.snoc (Ghost.reveal l, va'.contents)))
+        (list_iter_state p state a (array_of' wl') res (List.Tot.snoc (Ghost.reveal l, va'.contents)));
+      return res
+    )
+    a len (array_of' wl0) init
+  in
+  let _ = gen_elim () in
+  let al' = vpattern_replace (fun al' -> list_iter_state _ _ _ al' _ _) in
+  rewrite (list_iter_state p state a al' res wr0.contents) (list_iter_state0 p state a al' res wr0.contents);
+  let _ = gen_elim () in
+  rewrite (aparse (parse_list p) a _) (aparse (parse_list p) a va);
+  rewrite (state _ _) (state res va.contents);
+  return res
+
+#pop-options
+
+inline_for_extraction
+let list_iter_opt
+  (#k: parser_kind)
+  (#t: Type)
+  (#p: parser k t)
+  (j: jumper p)
+  (#t': Type)
+  (phi: Ghost.erased (t' -> t -> t'))
+  (state: t' -> list t -> vprop)
+  (f: (
+    (va: v k t { AP.length (array_of' va) > 0 }) ->
+    (a: byte_array) ->
+    (accu: t') ->
+    (l: Ghost.erased (list t)) ->
+    STT t'
+      (aparse p a va `star` state accu l)
+      (fun res -> aparse p a va `star` state res (List.Tot.snoc (Ghost.reveal l, va.contents)) `star` pure (res == Ghost.reveal phi accu va.contents))
+  ))
+  (#va: _)
+  (a: byte_array)
+  (len: SZ.size_t)
+  (init: t')
+: ST t'
+    (aparse_list p a va `star` state init [])
+    (fun res -> aparse_list p a va `star` state res va.contents)
+    (SZ.size_v len == length_opt va.array /\
+      k.parser_kind_subkind == Some ParserStrong
+    )
+    (fun res -> res == List.Tot.fold_left (Ghost.reveal phi) init va.contents)
+= let _ = ghost_is_cons_opt p a in
+  if len = SZ.zero_size
+  then begin
+    rewrite (state _ _) (state init va.contents);
+    return init
+  end else begin
+    let _ = elim_aparse_list_cons p a _ in
+    let res = list_iter j phi state f a len init in
+    let _ = intro_aparse_list_cons p a _ in
+    rewrite (aparse_list _ _ _) (aparse_list p a va);
+    rewrite (state _ _) (state res va.contents);
+    return res
+  end
+
+(*
+admit_ ();
+  return (magic ())
+
+let gres = ghost_elim_cons p a in
+  let _ = gen_elim () in
+  let res = hop_aparse_aparse j (parse_list p) a gres in
+  res
+
+
+(*
+let va' = elim_aparse (parse_list p) a in
+  parse_list_eq p (AP.contents_of va');
+  let a2 = AP.split a SZ.zero_size in
+  let _ = gen_elim () in
+  let _ = intro_aparse (parse_list p) a2 in
+  let _ = intro_nil p a in
+  return a2
+
+let list_split_nil_l
+  (#k: parser_kind)
+  (#t: Type)
+  (p: parser k t)
+  (#va: v parse_list_kind (list t))
+  (a: byte_array)
 : STT byte_array
     (aparse (parse_list p) a va)
-    (fun res -> exists_ (fun va1 -> exists_ (fun va2 ->
+    (fun res -> exists_ (fun (va1: v parse_list_kind (list t)) -> exists_ (fun (va2: v parse_list_kind (list t)) ->
       aparse (parse_list p) a va1 `star`
       aparse (parse_list p) res va2 `star` pure (
       AP.merge_into (array_of va1) (array_of va2) (array_of va) /\
@@ -317,7 +900,30 @@ let list_split_nil_l
   let _ = intro_nil p a in
   return a2
 
-#push-options "--z3rlimit 32" // not even enough without FStarLang/FStar#2584
+
+let list_iter_gen_prefix
+  (#t: Type)
+  (va: v parse_list_kind (list t))
+  (ar: byte_array)
+  (vr: v parse_list_kind (list t))
+  (vl: v parse_list_kind (list t))
+: Tot prop
+= 
+  AP.merge_into (array_of' vl) (array_of' vr) (array_of va) /\
+  vl.contents == va.contents
+
+
+(*
+= let a2 = list_split_nil_l p a in
+  let _ = gen_elim_dep () in // replacing with explicit elim_exists, elim_pure WILL NOT decrease rlimit
+  let res = list_iter' j phi state f a a2 len init in
+  let _ = gen_elim () in
+  List.Tot.append_nil_l va.contents; // FIXME: WHY WHY WHY?
+  rewrite (aparse (parse_list p) a _) (aparse (parse_list p) a va);
+  rewrite (state _ _) (state res va.contents);
+  return res
+*)
+
 
 let list_iter
   (#k: parser_kind)
